src/impl/TLS13.Impl.ConnectionState.LocalHandshake.fst
@@ -2640,7 +2640,8 @@ fn try_send_client_hello
       c.handshake.messages.client_hello
       st0.CS.cs_model.CS.model_handshake.CS.hs_client_hello);
     with old_client_hello_present old_l_random old_l_session_id old_l_server_name
-         old_l_key_share old_l_cipher_suites old_l_signature_schemes. _;
+         old_l_key_share old_l_p256_key_share old_l_cipher_suites
+         old_l_signature_schemes. _;
     unfold (client_hello_metadata_exactly
       c.handshake.messages.client_hello_has_server_name
       c.handshake.messages.client_hello_server_name_len
@@ -5198,7 +5199,7 @@ fn try_derive_server_shared_secret_from_private_array
     c.handshake.messages.client_hello_present
     c.handshake.messages.client_hello
     st0.CS.cs_model.CS.model_handshake.CS.hs_client_hello);
-  with ch_present ch_random ch_session_id ch_server_name ch_key_share ch_cipher_suites ch_signature_schemes. _;
+  with ch_present ch_random ch_session_id ch_server_name ch_key_share ch_p256_key_share ch_cipher_suites ch_signature_schemes. _;
 
   let ch = Ghost.hide (Some?.v st0.CS.cs_model.CS.model_handshake.CS.hs_client_hello);
   assert (pure (st0.CS.cs_model.CS.model_handshake.CS.hs_client_hello ==
